add rust bench

rust_benchmarks/lib.rs
@@ -1,0 +1,91 @@
+use vstd::prelude::*;
+
+#[cfg(feature = "base58")]
+gen!(
+    base58,
+    58,
+    b"ModueSymbhaswnPr123456789ABCDEFGHNRVfgctiUvzKqYTJkLxpZXjQW"
+);
+
+#[cfg(feature = "base62")]
+gen!(
+    base62,
+    62,
+    b"ModuleSymbhasOwnPr0123456789ABCDEFGHNRVfgctiUvzKqYTJkLxpZXIjQW"
+);
+
+#[cfg(feature = "base64")]
+gen!(
+    base64,
+    64,
+    b"ModuleSymbhasOwnPr-0123456789ABCDEFGHNRVfgctiUvz_KqYTJkLxpZXIjQW"
+);
+
+verus! {
+    macro_rules! gen {
+    ($mod:tt, $len:tt, $alphabet:tt) => {
+        #[doc = concat!(" Nanoid with alphabet table `", stringify!($alphabet), "`")]
+        mod $mod {
+            pub const MASK: usize = $len - 1;
+            pub const ALPHABET: &'static [u8; $len] = $alphabet;
+        }
+
+        #[doc = concat!(" Nanoid with ", stringify!($mod))]
+        #[must_use]
+        pub fn $mod<const N: usize>() -> String {
+            let mut bytes = [0u8; N];
+
+            getrandom::getrandom(&mut bytes)
+                .unwrap_or_else(|err| panic!("could not retreive random bytes: {err}"));
+
+            bytes
+                .iter_mut()
+                .for_each(|b| *b = $mod::ALPHABET[*b as usize & $mod::MASK]);
+
+            String::from_utf8_lossy(&bytes).to_string()
+        }
+    };
+}
+
+#[cfg(test)]
+mod tests {
+    use super::*;
+
+    #[test]
+    #[cfg(feature = "base58")]
+    fn generates_base58() {
+        let id = base58::<21>();
+        println!("{}", &id);
+        assert_eq!(id.len(), 21);
+    }
+
+    #[test]
+    #[cfg(feature = "base62")]
+    fn generates_base62() {
+        let id = base62::<21>();
+        println!("{}", &id);
+        assert_eq!(id.len(), 21);
+    }
+
+    #[test]
+    #[cfg(feature = "base64")]
+    fn generates_base64() {
+        let id = base64::<21>();
+        println!("{}", &id);
+        assert_eq!(id.len(), 21);
+    }
+
+    fn main() {
+        gen!(
+            uid,
+            64,
+            b"_-0123456789abcdefghijklmnopqrstuvwxyzABCDEFGHIJKLMNOPQRSTUVWXYZ"
+        );
+
+        let id = uid::<21>();
+        println!("{}", &id);
+        assert_eq!(id.len(), 21);
+    }
+}
+
+}
