rust_benchmarks/non-linear.rs
@@ -1,0 +1,63 @@
+use vstd::prelude::*;
+verus! {
+
+mod M1 {
+                use builtin::*;
+            
+                pub closed spec fn min(x: int, y: int) -> int {
+                    if x <= y {
+                        x
+                    } else {
+                        y
+                    }
+                }
+            
+                pub proof fn lemma_min(x: int, y: int)
+                    ensures
+                        min(x, y) <= x,
+                        min(x, y) <= y,
+                        min(x, y) == x || min(x, y) == y,
+                {
+                }
+            }
+            
+        mod M2 {
+                use builtin::*;
+                use crate::M1::*;
+            
+                fn test() {
+                    assert(min(10, 20) == 10) by {
+                        lemma_min(10, 20);
+                        lemma_min(100, 200);
+                    }
+                    assert(min(10, 20) == 10); // succeeds
+                  //  assert(min(100, 200) == 100); // FAILS
+                }
+            }
+            
+
+  proof fn bound_check(x: u32, y: u32, z: u32)
+        requires
+            x <= 0xffff,
+            y <= 0xffff,
+           // z <= 0xffff,
+    {
+        assert(x * y <= 0x100000000) by (nonlinear_arith)
+            requires
+                x <= 0xffff,
+                y <= 0xffff,
+            //    z <= 0xffff,
+        {
+            // nonlinear_arith proof block does not have any surrounding facts by default
+            // assert(z <= 0xffff);  <- Trivial, but fails since this property is not included in the `requires` clause
+            assert(x * y <= 0x100000000);
+        }
+    }
+
+    fn main() {
+        assert(1==1)
+
+    }
+
+    
+}
