rust_benchmarks/recurse_fail.rs
@@ -1,0 +1,37 @@
+use vstd::prelude::*;
+verus! {
+        spec fn triangle(n: nat) -> nat
+                decreases n,
+         {
+                if n == 0 {
+                        0
+                } else {
+                        n + triangle((n - 1) as nat)
+                }
+        }
+
+
+        fn rec_triangle(n: u32) -> u32
+                requires
+                triangle(n as nat) < 0x1_0000_0000,
+        {
+                let mut i = 0;
+                let n = 32;
+                while i < n {
+                        i += 1;
+                        if n == 0 {
+                         return 0 as u32;
+                        } else {
+                         return n + rec_triangle(n - 1) as u32; 
+                        }
+                        //return (i += 1) as u32;
+            }
+           return n
+        }
+    
+        fn main() {
+                //assert(triangle(2) == 3);
+                assert(forall|i: nat| triangle(i) >= 0);
+            }
+
+}
