rust_benchmarks/recurse_nospec.rs
@@ -1,0 +1,24 @@
+use vstd::prelude::*;
+verus! {
+
+
+        fn rec_triangle(n: u32)  -> u32
+                requires
+                 n < 0x1_0000_0000,
+
+        {
+                let mut i = 0;
+                while i < n {
+                        let sum =  n + rec_triangle(n - 1);
+                        n + rec_triangle(n - 1);
+                        assert(sum < 0x1_0000_0000);
+                        i += 1;
+                };
+                return i as u32;
+        }
+
+        fn main() {
+                let n = rec_triangle(3);
+            }
+
+}
