rust_benchmarks/recurse_success.rs
@@ -1,0 +1,32 @@
+use vstd::prelude::*;
+verus! {
+        spec fn triangle(n: nat) -> nat
+                decreases n,
+         {
+                if n == 0 {
+                        0
+                } else {
+                        n + triangle((n - 1) as nat)
+                }
+        }
+
+        fn rec_triangle(n: u32) -> (sum: u32)
+                requires
+                triangle(n as nat) < 0x1_0000_0000,
+                ensures
+                sum == triangle(n as nat),
+        {
+
+            if n == 0 {
+                0
+                } else {
+                n + rec_triangle(n - 1)
+                }
+        }
+    
+        fn main() {
+                //assert(triangle(2) == 3);
+                assert(forall|i: nat| triangle(i) >= 0);
+            }
+
+}
