timeout1.sol
@@ -26,9 +26,7 @@ contract Test {
         for (uint256 _i; _i < _tokens.length; _i++) {
                 indexTokens[_i] = (_weights[_i] * _xX96 * 10 ** _tokens[_i]) / _totalWeights;
                  assert(indexTokens[_i] >=  (_weights[_i] * _xX96 * 10 ** _tokens[_i]));
-        }
-       
-
+        }   
   }
    
 }
