corral_out.bpl
@@ -145,23 +145,24 @@ var _fundTokenIdx_Test: [Ref]Ref;
 
 var _isTokenInIndex_Test: [Ref]Ref;
 
-procedure {:public} culpritOne_Test(this: Ref, msgsender_MSG: Ref, msgvalue_MSG: int, _tokens_s130: Ref, _weights_s130: Ref, indexTokens_s130: Ref, FixedPoint96_s130: int);
+procedure {:public} culpritOne_Test(this: Ref, msgsender_MSG: Ref, msgvalue_MSG: int, _tokens_s302: Ref, _weights_s302: Ref, indexTokens_s302: Ref, FixedPoint96_s302: int);
   modifies _totalWeights_Test, M_int_int;
 
 
 
-implementation {:ForceInline} culpritOne_Test(this: Ref, msgsender_MSG: Ref, msgvalue_MSG: int, _tokens_s130: Ref, _weights_s130: Ref, indexTokens_s130: Ref, FixedPoint96_s130: int)
+implementation {:ForceInline} culpritOne_Test(this: Ref, msgsender_MSG: Ref, msgvalue_MSG: int, _tokens_s302: Ref, _weights_s302: Ref, indexTokens_s302: Ref, FixedPoint96_s302: int)
 {
-  var _i_s67: int;
-  var _xX96_s129: int;
-  var _i_s128: int;
+  var _i_s122: int;
+  var _xX96_s301: int;
+  var _i_s227: int;
+  var _i_s300: int;
 
   anon0:
     call {:si_unique_call 8} {:cexpr "_verisolFirstArg"} boogie_si_record_sol2Bpl_bool(false);
     call {:si_unique_call 9} {:cexpr "this"} boogie_si_record_sol2Bpl_ref(this);
     call {:si_unique_call 10} {:cexpr "msg.sender"} boogie_si_record_sol2Bpl_ref(msgsender_MSG);
     call {:si_unique_call 11} {:cexpr "msg.value"} boogie_si_record_sol2Bpl_int(msgvalue_MSG);
-    call {:si_unique_call 12} {:cexpr "FixedPoint96"} boogie_si_record_sol2Bpl_int(FixedPoint96_s130);
+    call {:si_unique_call 12} {:cexpr "FixedPoint96"} boogie_si_record_sol2Bpl_int(FixedPoint96_s302);
     call {:si_unique_call 13} {:cexpr "_verisolLastArg"} boogie_si_record_sol2Bpl_bool(true);
     goto corral_source_split_3;
 
@@ -169,136 +170,286 @@ implementation {:ForceInline} culpritOne_Test(this: Ref, msgsender_MSG: Ref, msg
     goto corral_source_split_4;
 
   corral_source_split_4:
-    assume Length[_tokens_s130] >= 0;
-    assume Length[_weights_s130] >= 0;
-    assume Length[_tokens_s130] == Length[_weights_s130];
+    assume Length[_tokens_s302] >= 0;
+    assume Length[_weights_s302] >= 0;
+    assume Length[_tokens_s302] == Length[_weights_s302];
     goto corral_source_split_5;
 
   corral_source_split_5:
-    assume _i_s67 >= 0;
-    assume Length[_tokens_s130] >= 0;
+    assume _i_s122 >= 0;
+    assume Length[_tokens_s302] >= 0;
     goto corral_source_split_6;
 
   corral_source_split_6:
-    havoc _i_s67;
-    goto anon4_LoopHead;
+    havoc _i_s122;
+    goto anon6_LoopHead;
 
-  anon4_LoopHead:
-    goto anon4_LoopDone, anon4_LoopBody;
+  anon6_LoopHead:
+    goto anon6_LoopDone, anon6_LoopBody;
 
-  anon4_LoopBody:
-    assume {:partition} _i_s67 < Length[_tokens_s130];
+  anon6_LoopBody:
+    assume {:partition} _i_s122 < Length[_tokens_s302];
     goto corral_source_split_8;
 
   corral_source_split_8:
     goto corral_source_split_9;
 
   corral_source_split_9:
-    assume _totalWeights_Test[this] >= 0;
-    assume _i_s67 >= 0;
-    assume M_int_int[_weights_s130][_i_s67] >= 0;
-    _totalWeights_Test[this] := _totalWeights_Test[this] + M_int_int[_weights_s130][_i_s67];
-    call {:si_unique_call 14} {:cexpr "_totalWeights"} boogie_si_record_sol2Bpl_int(_totalWeights_Test[this]);
+    assume _i_s122 >= 0;
+    assume M_int_int[_tokens_s302][_i_s122] >= 0;
+    assert M_int_int[_tokens_s302][_i_s122] >= 0;
     goto corral_source_split_10;
 
   corral_source_split_10:
-    assume _i_s67 >= 0;
-    assume M_int_int[_tokens_s130][_i_s67] >= 0;
-    assume M_int_int[_fundTokenIdx_Test[this]][M_int_int[_tokens_s130][_i_s67]] >= 0;
-    assume _i_s67 >= 0;
-    M_int_int[_fundTokenIdx_Test[this]][M_int_int[_tokens_s130][_i_s67]] := _i_s67;
-    call {:si_unique_call 15} {:cexpr "_fundTokenIdx[_tokens[_i]]"} boogie_si_record_sol2Bpl_int(M_int_int[_fundTokenIdx_Test[this]][M_int_int[_tokens_s130][_i_s67]]);
+    assume _totalWeights_Test[this] >= 0;
+    assume _i_s122 >= 0;
+    assume M_int_int[_weights_s302][_i_s122] >= 0;
+    _totalWeights_Test[this] := _totalWeights_Test[this] + M_int_int[_weights_s302][_i_s122];
+    call {:si_unique_call 14} {:cexpr "_totalWeights"} boogie_si_record_sol2Bpl_int(_totalWeights_Test[this]);
     goto corral_source_split_11;
 
   corral_source_split_11:
-    assume _i_s67 >= 0;
-    assume M_int_int[_tokens_s130][_i_s67] >= 0;
-    assume M_int_int[_isTokenInIndex_Test[this]][M_int_int[_tokens_s130][_i_s67]] >= 0;
-    M_int_int[_isTokenInIndex_Test[this]][M_int_int[_tokens_s130][_i_s67]] := 1;
-    call {:si_unique_call 16} {:cexpr "_isTokenInIndex[_tokens[_i]]"} boogie_si_record_sol2Bpl_int(M_int_int[_isTokenInIndex_Test[this]][M_int_int[_tokens_s130][_i_s67]]);
+    assume _i_s122 >= 0;
+    assume M_int_int[_weights_s302][_i_s122] >= 0;
+    assume _totalWeights_Test[this] >= 0;
+    assume _totalWeights_Test[this] >= 0;
+    assume _i_s122 >= 0;
+    assume M_int_int[_weights_s302][_i_s122] >= 0;
+    assume _i_s122 >= 0;
+    assume M_int_int[_tokens_s302][_i_s122] >= 0;
+    assume M_int_int[_tokens_s302][_i_s122] >= 0;
+    assert M_int_int[_weights_s302][_i_s122] <= _totalWeights_Test[this] && _totalWeights_Test[this] <= M_int_int[_tokens_s302][_i_s122];
     goto corral_source_split_12;
 
   corral_source_split_12:
-    assume _i_s67 >= 0;
-    _i_s67 := _i_s67 + 1;
-    call {:si_unique_call 17} {:cexpr "_i"} boogie_si_record_sol2Bpl_int(_i_s67);
-    assume _i_s67 >= 0;
-    goto anon4_LoopHead;
+    assume _i_s122 >= 0;
+    assume M_int_int[_tokens_s302][_i_s122] >= 0;
+    assume M_int_int[_fundTokenIdx_Test[this]][M_int_int[_tokens_s302][_i_s122]] >= 0;
+    assume _i_s122 >= 0;
+    M_int_int[_fundTokenIdx_Test[this]][M_int_int[_tokens_s302][_i_s122]] := _i_s122;
+    call {:si_unique_call 15} {:cexpr "_fundTokenIdx[_tokens[_i]]"} boogie_si_record_sol2Bpl_int(M_int_int[_fundTokenIdx_Test[this]][M_int_int[_tokens_s302][_i_s122]]);
+    goto corral_source_split_13;
 
-  anon4_LoopDone:
-    assume {:partition} Length[_tokens_s130] <= _i_s67;
-    goto anon2;
-
-  anon2:
-    assume _xX96_s129 >= 0;
-    assume FixedPoint96_s130 >= 0;
-    assume _totalWeights_Test[this] >= 0;
-    assume FixedPoint96_s130 + _totalWeights_Test[this] >= 0;
-    assume M_int_int[_weights_s130][0] >= 0;
-    assume FixedPoint96_s130 + _totalWeights_Test[this] - M_int_int[_weights_s130][0] >= 0;
-    _xX96_s129 := FixedPoint96_s130 + _totalWeights_Test[this] - M_int_int[_weights_s130][0];
-    call {:si_unique_call 18} {:cexpr "_xX96"} boogie_si_record_sol2Bpl_int(_xX96_s129);
+  corral_source_split_13:
+    assume _i_s122 >= 0;
+    assume M_int_int[_tokens_s302][_i_s122] >= 0;
+    assume M_int_int[_fundTokenIdx_Test[this]][M_int_int[_tokens_s302][_i_s122]] >= 0;
+    assert M_int_int[_fundTokenIdx_Test[this]][M_int_int[_tokens_s302][_i_s122]] >= 0;
     goto corral_source_split_14;
 
   corral_source_split_14:
-    assume _i_s128 >= 0;
-    assume Length[_tokens_s130] >= 0;
+    assume _i_s122 >= 0;
+    assume M_int_int[_tokens_s302][_i_s122] >= 0;
+    assume M_int_int[_isTokenInIndex_Test[this]][M_int_int[_tokens_s302][_i_s122]] >= 0;
+    M_int_int[_isTokenInIndex_Test[this]][M_int_int[_tokens_s302][_i_s122]] := 1;
+    call {:si_unique_call 16} {:cexpr "_isTokenInIndex[_tokens[_i]]"} boogie_si_record_sol2Bpl_int(M_int_int[_isTokenInIndex_Test[this]][M_int_int[_tokens_s302][_i_s122]]);
     goto corral_source_split_15;
 
   corral_source_split_15:
-    havoc _i_s128;
-    goto anon5_LoopHead;
+    assume _i_s122 >= 0;
+    assume M_int_int[_tokens_s302][_i_s122] >= 0;
+    assume M_int_int[_isTokenInIndex_Test[this]][M_int_int[_tokens_s302][_i_s122]] >= 0;
+    assume _i_s122 >= 0;
+    assume M_int_int[_weights_s302][_i_s122] >= 0;
+    assert M_int_int[_isTokenInIndex_Test[this]][M_int_int[_tokens_s302][_i_s122]] == M_int_int[_weights_s302][_i_s122];
+    goto corral_source_split_16;
 
-  anon5_LoopHead:
-    goto anon5_LoopDone, anon5_LoopBody;
-
-  anon5_LoopBody:
-    assume {:partition} _i_s128 < Length[_tokens_s130];
+  corral_source_split_16:
+    assume FixedPoint96_s302 >= 0;
+    call {:si_unique_call 17} culpritOne_Test(this, msgsender_MSG, msgvalue_MSG, _tokens_s302, _weights_s302, indexTokens_s302, FixedPoint96_s302);
     goto corral_source_split_17;
 
   corral_source_split_17:
-    goto corral_source_split_18;
+    assume _i_s122 >= 0;
+    _i_s122 := _i_s122 + 1;
+    call {:si_unique_call 18} {:cexpr "_i"} boogie_si_record_sol2Bpl_int(_i_s122);
+    assume _i_s122 >= 0;
+    goto anon6_LoopHead;
 
-  corral_source_split_18:
-    assume _i_s128 >= 0;
-    assume M_int_int[indexTokens_s130][_i_s128] >= 0;
-    assume _i_s128 >= 0;
-    assume M_int_int[_weights_s130][_i_s128] >= 0;
-    assume _xX96_s129 >= 0;
-    assume M_int_int[_weights_s130][_i_s128] + _xX96_s129 >= 0;
-    assume M_int_int[_weights_s130][_i_s128] + _xX96_s129 + 10 >= 0;
-    assume _i_s128 >= 0;
-    assume M_int_int[_tokens_s130][_i_s128] >= 0;
-    assume M_int_int[_weights_s130][_i_s128] + _xX96_s129 + 10 + M_int_int[_tokens_s130][_i_s128] >= 0;
-    assume _totalWeights_Test[this] >= 0;
-    assume M_int_int[_weights_s130][_i_s128] + _xX96_s129 + 10 + M_int_int[_tokens_s130][_i_s128] - _totalWeights_Test[this] >= 0;
-    M_int_int[indexTokens_s130][_i_s128] := M_int_int[_weights_s130][_i_s128] + _xX96_s129 + 10 + M_int_int[_tokens_s130][_i_s128] - _totalWeights_Test[this];
-    call {:si_unique_call 19} {:cexpr "indexTokens[_i]"} boogie_si_record_sol2Bpl_int(M_int_int[indexTokens_s130][_i_s128]);
+  anon6_LoopDone:
+    assume {:partition} Length[_tokens_s302] <= _i_s122;
+    goto anon2;
+
+  anon2:
+    assume M_int_int[_weights_s302][0] >= 0;
+    assert M_int_int[_weights_s302][0] > 0;
     goto corral_source_split_19;
 
   corral_source_split_19:
-    assume _i_s128 >= 0;
-    assume M_int_int[indexTokens_s130][_i_s128] >= 0;
-    assume _i_s128 >= 0;
-    assume M_int_int[_weights_s130][_i_s128] >= 0;
-    assume _xX96_s129 >= 0;
-    assume M_int_int[_weights_s130][_i_s128] + _xX96_s129 >= 0;
-    assume M_int_int[_weights_s130][_i_s128] + _xX96_s129 + 10 >= 0;
-    assume _i_s128 >= 0;
-    assume M_int_int[_tokens_s130][_i_s128] >= 0;
-    assume M_int_int[_weights_s130][_i_s128] + _xX96_s129 + 10 + M_int_int[_tokens_s130][_i_s128] >= 0;
-    assert M_int_int[indexTokens_s130][_i_s128] >= M_int_int[_weights_s130][_i_s128] + _xX96_s129 + 10 + M_int_int[_tokens_s130][_i_s128];
+    assume _xX96_s301 >= 0;
+    assume FixedPoint96_s302 >= 0;
+    assume _totalWeights_Test[this] >= 0;
+    assume FixedPoint96_s302 * _totalWeights_Test[this] >= 0;
+    assume M_int_int[_weights_s302][0] >= 0;
+    assume FixedPoint96_s302 * _totalWeights_Test[this] div M_int_int[_weights_s302][0] >= 0;
+    _xX96_s301 := FixedPoint96_s302 * _totalWeights_Test[this] div M_int_int[_weights_s302][0];
+    call {:si_unique_call 19} {:cexpr "_xX96"} boogie_si_record_sol2Bpl_int(_xX96_s301);
     goto corral_source_split_20;
 
   corral_source_split_20:
-    assume _i_s128 >= 0;
-    _i_s128 := _i_s128 + 1;
-    call {:si_unique_call 20} {:cexpr "_i"} boogie_si_record_sol2Bpl_int(_i_s128);
-    assume _i_s128 >= 0;
-    goto anon5_LoopHead;
+    assume _xX96_s301 >= 0;
+    assert _xX96_s301 > 0;
+    goto corral_source_split_21;
 
-  anon5_LoopDone:
-    assume {:partition} Length[_tokens_s130] <= _i_s128;
+  corral_source_split_21:
+    assume Length[_tokens_s302] >= 0;
+    assert Length[_tokens_s302] > 0;
+    goto corral_source_split_22;
+
+  corral_source_split_22:
+    assume _i_s227 >= 0;
+    assume Length[_tokens_s302] >= 0;
+    goto corral_source_split_23;
+
+  corral_source_split_23:
+    havoc _i_s227;
+    goto anon7_LoopHead;
+
+  anon7_LoopHead:
+    goto anon7_LoopDone, anon7_LoopBody;
+
+  anon7_LoopBody:
+    assume {:partition} _i_s227 < Length[_tokens_s302];
+    goto corral_source_split_25;
+
+  corral_source_split_25:
+    goto corral_source_split_26;
+
+  corral_source_split_26:
+    assume _totalWeights_Test[this] >= 0;
+    assert _totalWeights_Test[this] != 0;
+    goto corral_source_split_27;
+
+  corral_source_split_27:
+    assume _i_s227 >= 0;
+    assume M_int_int[indexTokens_s302][_i_s227] >= 0;
+    assume _i_s227 >= 0;
+    assume M_int_int[_weights_s302][_i_s227] >= 0;
+    assume _xX96_s301 >= 0;
+    assume M_int_int[_weights_s302][_i_s227] * _xX96_s301 >= 0;
+    assume _i_s227 >= 0;
+    assume M_int_int[_tokens_s302][_i_s227] >= 0;
+    assume M_int_int[_tokens_s302][_i_s227] >= 0;
+    assume M_int_int[_weights_s302][_i_s227] * _xX96_s301 * M_int_int[_tokens_s302][_i_s227] >= 0;
+    assume _totalWeights_Test[this] >= 0;
+    assume M_int_int[_weights_s302][_i_s227] * _xX96_s301 * M_int_int[_tokens_s302][_i_s227] div _totalWeights_Test[this] >= 0;
+    M_int_int[indexTokens_s302][_i_s227] := M_int_int[_weights_s302][_i_s227] * _xX96_s301 * M_int_int[_tokens_s302][_i_s227] div _totalWeights_Test[this];
+    call {:si_unique_call 20} {:cexpr "indexTokens[_i]"} boogie_si_record_sol2Bpl_int(M_int_int[indexTokens_s302][_i_s227]);
+    goto corral_source_split_28;
+
+  corral_source_split_28:
+    assume _i_s227 >= 0;
+    assume M_int_int[_weights_s302][_i_s227] >= 0;
+    assume _xX96_s301 >= 0;
+    assume M_int_int[_weights_s302][_i_s227] * _xX96_s301 >= 0;
+    assume _i_s227 >= 0;
+    assume M_int_int[_tokens_s302][_i_s227] >= 0;
+    assume M_int_int[_tokens_s302][_i_s227] >= 0;
+    assume M_int_int[_weights_s302][_i_s227] * _xX96_s301 * M_int_int[_tokens_s302][_i_s227] >= 0;
+    assert M_int_int[_weights_s302][_i_s227] * _xX96_s301 * M_int_int[_tokens_s302][_i_s227] > 0;
+    goto corral_source_split_29;
+
+  corral_source_split_29:
+    assume _i_s227 >= 0;
+    assume M_int_int[indexTokens_s302][_i_s227] >= 0;
+    assume _i_s227 >= 0;
+    assume M_int_int[_weights_s302][_i_s227] >= 0;
+    assume _xX96_s301 >= 0;
+    assume M_int_int[_weights_s302][_i_s227] * _xX96_s301 >= 0;
+    assume _i_s227 >= 0;
+    assume M_int_int[_tokens_s302][_i_s227] >= 0;
+    assume M_int_int[_tokens_s302][_i_s227] >= 0;
+    assume M_int_int[_weights_s302][_i_s227] * _xX96_s301 * M_int_int[_tokens_s302][_i_s227] >= 0;
+    assert M_int_int[indexTokens_s302][_i_s227] >= M_int_int[_weights_s302][_i_s227] * _xX96_s301 * M_int_int[_tokens_s302][_i_s227];
+    goto corral_source_split_30;
+
+  corral_source_split_30:
+    assume _i_s227 >= 0;
+    _i_s227 := _i_s227 + 1;
+    call {:si_unique_call 21} {:cexpr "_i"} boogie_si_record_sol2Bpl_int(_i_s227);
+    assume _i_s227 >= 0;
+    goto anon7_LoopHead;
+
+  anon7_LoopDone:
+    assume {:partition} Length[_tokens_s302] <= _i_s227;
+    goto anon4;
+
+  anon4:
+    assume _i_s300 >= 0;
+    assume Length[_tokens_s302] >= 0;
+    goto corral_source_split_32;
+
+  corral_source_split_32:
+    havoc _i_s300;
+    goto anon8_LoopHead;
+
+  anon8_LoopHead:
+    goto anon8_LoopDone, anon8_LoopBody;
+
+  anon8_LoopBody:
+    assume {:partition} _i_s300 < Length[_tokens_s302];
+    goto corral_source_split_34;
+
+  corral_source_split_34:
+    goto corral_source_split_35;
+
+  corral_source_split_35:
+    assume _totalWeights_Test[this] >= 0;
+    assert _totalWeights_Test[this] != 0;
+    goto corral_source_split_36;
+
+  corral_source_split_36:
+    assume _i_s300 >= 0;
+    assume M_int_int[indexTokens_s302][_i_s300] >= 0;
+    assume _i_s300 >= 0;
+    assume M_int_int[_weights_s302][_i_s300] >= 0;
+    assume _xX96_s301 >= 0;
+    assume M_int_int[_weights_s302][_i_s300] * _xX96_s301 >= 0;
+    assume _i_s300 >= 0;
+    assume M_int_int[_tokens_s302][_i_s300] >= 0;
+    assume M_int_int[_tokens_s302][_i_s300] >= 0;
+    assume M_int_int[_weights_s302][_i_s300] * _xX96_s301 * M_int_int[_tokens_s302][_i_s300] >= 0;
+    assume _totalWeights_Test[this] >= 0;
+    assume M_int_int[_weights_s302][_i_s300] * _xX96_s301 * M_int_int[_tokens_s302][_i_s300] div _totalWeights_Test[this] >= 0;
+    M_int_int[indexTokens_s302][_i_s300] := M_int_int[_weights_s302][_i_s300] * _xX96_s301 * M_int_int[_tokens_s302][_i_s300] div _totalWeights_Test[this];
+    call {:si_unique_call 22} {:cexpr "indexTokens[_i]"} boogie_si_record_sol2Bpl_int(M_int_int[indexTokens_s302][_i_s300]);
+    goto corral_source_split_37;
+
+  corral_source_split_37:
+    assume _i_s300 >= 0;
+    assume M_int_int[_weights_s302][_i_s300] >= 0;
+    assume _xX96_s301 >= 0;
+    assume M_int_int[_weights_s302][_i_s300] * _xX96_s301 >= 0;
+    assume _i_s300 >= 0;
+    assume M_int_int[_tokens_s302][_i_s300] >= 0;
+    assume M_int_int[_tokens_s302][_i_s300] >= 0;
+    assume M_int_int[_weights_s302][_i_s300] * _xX96_s301 * M_int_int[_tokens_s302][_i_s300] >= 0;
+    assert M_int_int[_weights_s302][_i_s300] * _xX96_s301 * M_int_int[_tokens_s302][_i_s300] > 0;
+    goto corral_source_split_38;
+
+  corral_source_split_38:
+    assume _i_s300 >= 0;
+    assume M_int_int[indexTokens_s302][_i_s300] >= 0;
+    assume _i_s300 >= 0;
+    assume M_int_int[_weights_s302][_i_s300] >= 0;
+    assume _xX96_s301 >= 0;
+    assume M_int_int[_weights_s302][_i_s300] * _xX96_s301 >= 0;
+    assume _i_s300 >= 0;
+    assume M_int_int[_tokens_s302][_i_s300] >= 0;
+    assume M_int_int[_tokens_s302][_i_s300] >= 0;
+    assume M_int_int[_weights_s302][_i_s300] * _xX96_s301 * M_int_int[_tokens_s302][_i_s300] >= 0;
+    assert M_int_int[indexTokens_s302][_i_s300] >= M_int_int[_weights_s302][_i_s300] * _xX96_s301 * M_int_int[_tokens_s302][_i_s300];
+    goto corral_source_split_39;
+
+  corral_source_split_39:
+    assume _i_s300 >= 0;
+    _i_s300 := _i_s300 + 1;
+    call {:si_unique_call 23} {:cexpr "_i"} boogie_si_record_sol2Bpl_int(_i_s300);
+    assume _i_s300 >= 0;
+    goto anon8_LoopHead;
+
+  anon8_LoopDone:
+    assume {:partition} Length[_tokens_s302] <= _i_s300;
     return;
 }
 
@@ -330,20 +481,20 @@ implementation CorralChoice_Test(this: Ref)
   var msgsender_MSG: Ref;
   var msgvalue_MSG: int;
   var choice: int;
-  var _tokens_s130: Ref;
-  var _weights_s130: Ref;
-  var indexTokens_s130: Ref;
-  var FixedPoint96_s130: int;
+  var _tokens_s302: Ref;
+  var _weights_s302: Ref;
+  var indexTokens_s302: Ref;
+  var FixedPoint96_s302: int;
   var tmpNow: int;
 
   anon0:
     havoc msgsender_MSG;
     havoc msgvalue_MSG;
     havoc choice;
-    havoc _tokens_s130;
-    havoc _weights_s130;
-    havoc indexTokens_s130;
-    havoc FixedPoint96_s130;
+    havoc _tokens_s302;
+    havoc _weights_s302;
+    havoc indexTokens_s302;
+    havoc FixedPoint96_s302;
     havoc tmpNow;
     tmpNow := now;
     havoc now;
@@ -355,10 +506,10 @@ implementation CorralChoice_Test(this: Ref)
 
   anon2_Then:
     assume {:partition} choice == 1;
-    call {:si_unique_call 21} _tokens_s130 := FreshRefGenerator();
-    call {:si_unique_call 22} _weights_s130 := FreshRefGenerator();
-    call {:si_unique_call 23} indexTokens_s130 := FreshRefGenerator();
-    call {:si_unique_call 24} culpritOne_Test(this, msgsender_MSG, msgvalue_MSG, _tokens_s130, _weights_s130, indexTokens_s130, FixedPoint96_s130);
+    call {:si_unique_call 24} _tokens_s302 := FreshRefGenerator();
+    call {:si_unique_call 25} _weights_s302 := FreshRefGenerator();
+    call {:si_unique_call 26} indexTokens_s302 := FreshRefGenerator();
+    call {:si_unique_call 27} culpritOne_Test(this, msgsender_MSG, msgvalue_MSG, _tokens_s302, _weights_s302, indexTokens_s302, FixedPoint96_s302);
     return;
 
   anon2_Else:
@@ -380,10 +531,10 @@ implementation CorralEntry_Test()
   var msgvalue_MSG: int;
 
   anon0:
-    call {:si_unique_call 25} this := FreshRefGenerator();
+    call {:si_unique_call 28} this := FreshRefGenerator();
     assume now >= 0;
     assume DType[this] == Test;
-    call {:si_unique_call 26} Test_Test(this, msgsender_MSG, msgvalue_MSG);
+    call {:si_unique_call 29} Test_Test(this, msgsender_MSG, msgvalue_MSG);
     goto anon2_LoopHead;
 
   anon2_LoopHead:
@@ -391,7 +542,7 @@ implementation CorralEntry_Test()
 
   anon2_LoopBody:
     assume {:partition} true;
-    call {:si_unique_call 27} CorralChoice_Test(this);
+    call {:si_unique_call 30} CorralChoice_Test(this);
     goto anon2_LoopHead;
 
   anon2_LoopDone:
